add idea

src/MC_CTL.v
@@ -1,31 +1,20 @@
-Definition cAX: forall X : Type, 
-(X -> X -> Prop) -> (X -> Prop) -> X -> Prop := 
-  fun (X : Type) (e : X -> X -> Prop) (p : X -> Prop) (w : X) =>
-  forall v : X, e w v -> p v.
+Definition cAX (st : Type) (trans : st -> st -> Prop) (pred : st -> Prop) (w : st):= 
+forall v : st, trans w v -> pred v.
 
-Definition path: forall X : Type, (X -> X -> Prop) -> (nat -> X) -> Prop := 
-fun (X : Type) (e : X -> X -> Prop) (pi : nat -> X) =>
-forall n : nat, e (pi n) (pi (S n)).
+Definition path(st : Type) (trans : st -> st -> Prop) (pi : nat -> st):= 
+forall n : nat, trans (pi n) (pi (S n)).
 
-Definition p_until: forall X : Type,
-(X -> Prop) -> (X -> Prop) -> (nat -> X) -> Prop := 
-  fun (X : Type) (p q : X -> Prop) (pi : nat -> X) =>
-  exists2 n : nat, forall m : nat, m < n -> p (pi m) & q (pi n).
+Definition p_until(st : Type) (pred1 pred2 : st -> Prop) (pi : nat -> st):= 
+exists2 n : nat, forall m : nat, m < n -> pred1 (pi m) & pred2 (pi n).
 
-Definition p_release: forall X : Type, 
-(X -> Prop) -> (X -> Prop) -> (nat -> X) -> Prop := 
-  fun (X : Type) (p q : X -> Prop) (pi : nat -> X) =>
-  forall n : nat, (exists2 m : nat, m < n & p (pi m)) \/ q (pi n).
+Definition p_release(st : Type) (pred1 pred2 : st -> Prop) (pi : nat -> st):= 
+forall n : nat, (exists2 m : nat, m < n & pred1 (pi m)) \/ pred2 (pi n).
 
-Definition pAU : forall X : Type,
-(X -> X -> Prop) -> (X -> Prop) -> (X -> Prop) -> X -> Prop := 
-  fun (X : Type) (e : X -> X -> Prop) (p q : X -> Prop) (w : X) =>
-  forall pi : nat -> X, path X e pi -> (pi 0 = w) -> p_until X p q pi.
+Definition pAU (st : Type) (trans : st -> st -> Prop) (pred1 pred2 : st -> Prop) (w : st):= 
+forall pi : nat -> st, path st trans pi -> (pi 0 = w) -> p_until st pred1 pred2 pi.
 
-Definition pAR: forall X : Type,
-(X -> X -> Prop) -> (X -> Prop) -> (X -> Prop) -> X -> Prop := 
-fun (X : Type) (e : X -> X -> Prop) (p q : X -> Prop) (w : X) =>
-forall pi : nat -> X, path X e pi -> (pi 0 = w) -> p_release X p q pi.
+Definition pAR (st : Type) (trans : st -> st -> Prop) (pred1 pred2: st -> Prop) (w : st) := 
+forall pi : nat -> st, path st trans pi -> (pi 0 = w) -> p_release st pred1 pred2 pi.
 
 
 Inductive form : Set :=
